Add naturality law for MonadError

theories/Classes/Monad.v
@@ -10,15 +10,18 @@ Class Monad m : Type :=
 Arguments pure {m _ a} _.
 Arguments bind {m _ a b} _ _.
 
+Infix ">>=" := bind (at level 50, left associativity).
+Notation "u >> v" := (bind u (fun _ => v)) (at level 50, left associativity).
+
+Definition mapM {m} `{Monad m} {a b : Type} (f : a -> b) (u : m a) : m b :=
+  u >>= fun x => pure (f x).
+
 Class LawfulMonad m `{Monad m} : Prop :=
   { bind_pure_l : forall a b (x : a) (k : a -> m b), bind (pure x) k = k x
   ; bind_pure_r : forall a (u : m a), bind u pure = u
   ; bind_assoc : forall a b c (u : m a) (k : a -> m b) (h : b -> m c),
       bind (bind u k) h = bind u (fun x => bind (k x) h)
   }.
-
-Infix ">>=" := bind (at level 50, left associativity).
-Notation "u >> v" := (bind u (fun _ => v)) (at level 50, left associativity).
 
 (** In theory, the laws are part of the definition of a "monad",
     so [LawfulMonad] is what should really be named [Monad], and the record
